theories/theories/utp_reactive.thy
@@ -10,19 +10,18 @@ theory utp_reactive
 imports 
   utp_designs
   utp_theory
-  Sublist
 begin
 
-class REACTIVE_SORT = BOOL_SORT + LIST_SORT + FSET_SORT + STRING_SORT 
-                    + LESS_EQ_SORT + MINUS_SORT
+class REACTIVE_SORT = BOOL_SORT + LIST_SORT + FSET_SORT + STRING_LIST_SORT + MINUS_SORT
 
 default_sort REACTIVE_SORT
 
 abbreviation "wait \<equiv> MkPlain ''wait'' (BoolType) True"
-abbreviation "tr   \<equiv> MkPlain ''tr'' (ListType StringType) True"
+abbreviation tr :: "'a::REACTIVE_SORT VAR" where
+"tr   \<equiv> MkPlain ''tr'' (ListType StringType) True"
 
 definition SkipREA :: "'a WF_PREDICATE" where
-"SkipREA = `(\<not> ok \<and> ($tr \<le> $tr\<acute>)) \<or> (ok\<acute> \<and> ($tr\<acute> = $tr) \<and> II\<^bsub>REL_VAR - OKAY\<^esub>)`"
+"SkipREA = `(\<not> ok \<and> ($tr \<le> $tr\<acute>)) \<or> (ok\<acute> \<and> II\<^bsub>REL_VAR - OKAY\<^esub>)`"
 
 syntax 
   "_upred_skiprea" :: "upred" ("II\<^bsub>rea\<^esub>")
@@ -38,5 +37,41 @@ definition R2 :: "'a WF_PREDICATE \<Rightarrow> 'a WF_PREDICATE" where
 
 definition R3 :: "'a WF_PREDICATE \<Rightarrow> 'a WF_PREDICATE" where
 "R3(P) = `II\<^bsub>rea\<^esub> \<lhd> $wait \<rhd> P`"
+
+abbreviation "R \<equiv> R1 \<circ> R2 \<circ> R3"
+
+syntax
+  "_uexpr_subste"       :: "uexpr \<Rightarrow> uexpr \<Rightarrow> 'a VAR \<Rightarrow> uexpr" ("(_[_'/_])" [999,999] 1000)
+
+translations
+  "_uexpr_subste e v x" == "CONST SubstE e v x"
+
+lemma SubstP_ExprP [usubst]:
+  "(ExprP e)[v|x] = ExprP (e[v|x])"
+  by (utp_pred_tac, utp_expr_tac)
+
+lemma SkipREA_CondR_SkipR: 
+  "`II\<^bsub>rea\<^esub>` = `II \<lhd> ok \<rhd> ($tr \<le> $tr\<acute>)`"
+proof -
+
+  have "`II \<lhd> ok \<rhd> ($tr \<le> $tr\<acute>)` = `($okay\<acute> = $okay \<and> II\<^bsub>REL_VAR - OKAY\<^esub>) \<lhd> ok \<rhd> ($tr \<le> $tr\<acute>)`"
+    by (metis Diff_cancel ExistsP_empty HOMOGENEOUS_REL_VAR MkPlain_UNDASHED SkipRA.rep_eq SkipRA_unfold UnCI hom_alphabet_undash)
+
+  also have "... = `($okay\<acute> = $okay \<and> II\<^bsub>REL_VAR - OKAY\<^esub>)[true/okay] \<lhd> $okay \<rhd> (($tr \<le> $tr\<acute>)[false/okay])`"
+    by (rule CondR_VarP_aux, simp_all add:typing defined)
+
+  also have "... = `(ok \<and> II\<^bsub>REL_VAR - OKAY\<^esub>) \<lhd> ok \<rhd> ($tr \<le> $tr\<acute>)`"
+  proof -
+
+    have "(ulesseq :: 'b \<Rightarrow> 'b \<Rightarrow> 'b) \<in> FUNC2 (ListType StringType) (ListType StringType) BoolType"
+      by (simp add: closure) 
+
+    thus ?thesis
+      apply (insert SubstE_Op2E[of "VarE tr :: 'b WF_EXPRESSION" "ListType StringType" "VarE tr\<acute>" "ListType StringType" "ulesseq" BoolType "FalseE" "okay"])
+
+    apply (simp add:usubst typing defined closure var_simps)
+
+
+  oops (* FIXME: Can't finish the step without more laws about prefix *)
 
 end
