theories/laws/utp_subst_laws.thy
@@ -209,6 +209,33 @@ done
 
 subsection {* Expression Substitution Laws *}
 
+lemma SubstE_LitE [usubst]:
+  "v : a \<Longrightarrow> LitE v[e|x] = LitE v"
+  by (utp_expr_tac)
+
+(* Hmmmm, why does this proof take so much effort? It should just go through by
+   utp_expr_tac but I have to explicitly guide application of EvalE_Op1E. I think
+   there may be too much non-determinism. *)
+lemma SubstE_Op1E [usubst]:
+  "\<lbrakk> v :\<^sub>e a; f \<in> FUNC1 a b; e :\<^sub>e vtype x \<rbrakk> \<Longrightarrow> (Op1E f v)[e|x] = Op1E f (v[e|x])"
+  apply (auto simp add:evale typing defined)
+  apply (insert SubstE_type[of e x v a])
+  apply (simp)
+  apply (drule_tac ?b1.0="ba" and f="f" in EvalE_Op1E) back back
+  apply (simp_all)
+  apply (utp_expr_tac)
+done
+
+lemma SubstE_Op2E [usubst]:
+  "\<lbrakk> v1 :\<^sub>e a; v2 :\<^sub>e b; f \<in> FUNC2 a b c; e :\<^sub>e vtype x \<rbrakk> \<Longrightarrow> 
+     (Op2E f v1 v2)[e|x] = Op2E f (v1[e|x]) (v2[e|x])"
+  apply (auto simp add:evale typing defined)
+  apply (insert SubstE_type[of e x v1 a])
+  apply (insert SubstE_type[of e x v2 b])
+  apply (simp_all)
+  apply (metis EvalE_def Op2E_rep_eq SubstE.rep_eq)
+done
+
 lemma SubstE_TrueE [usubst]:
   "TrueE[e|x] = TrueE"
   by (utp_expr_tac)
