theories/tactics/utp_expr_tac.thy
@@ -70,6 +70,14 @@ theorem EvalE_LitE [evale] :
 "v : t \<Longrightarrow> \<lbrakk>LitE v\<rbrakk>\<epsilon>b = v"
   by (auto simp add: LitE_rep_eq EvalE_def)
 
+theorem EvalE_Op1E [evale] :
+"\<lbrakk> x :\<^sub>e a; f \<in> FUNC1 a b \<rbrakk> \<Longrightarrow> \<lbrakk>Op1E f x\<rbrakk>\<epsilon>b1 = f (\<lbrakk>x\<rbrakk>\<epsilon>b1)"
+  by (auto simp add: Op1E_rep_eq EvalE_def)
+
+theorem EvalE_Op2E [evale] :
+"\<lbrakk> x :\<^sub>e a; y :\<^sub>e b; f \<in> FUNC2 a b c \<rbrakk> \<Longrightarrow> \<lbrakk>Op2E f x y\<rbrakk>\<epsilon>b1 = f (\<lbrakk>x\<rbrakk>\<epsilon>b1) (\<lbrakk>y\<rbrakk>\<epsilon>b1)"
+  by (auto simp add: Op2E_rep_eq EvalE_def)
+
 theorem EvalE_DefaultE [evale] :
 "\<lbrakk>DefaultE t\<rbrakk>\<epsilon>b = default t"
   by (auto simp add: DefaultE_def EvalE_def LitE_rep_eq)
